coq/assoc_spec.v
@@ -32,6 +32,9 @@ Qed.
 
 Definition CircleArrayZ := ArrayZ.
 
+Function hash (k:Z): Z :=
+  if (Z.ltb k 0) then (Z.rem k 100) + 99 else (Z.rem k 100).
+
 Function caPut (arr: CircleArrayZ) (k:Z) (v:Z) : CircleArrayZ :=
   arrPut arr (Zmod k 100) v.
 
@@ -55,3 +58,51 @@ apply getput2.
 assumption.
 Qed.
 
+Lemma Zero_le_hash: forall k, 0 <= hash k.
+Proof.
+  intro.
+  unfold hash.
+  destruct k;simpl.
+  - apply Z.rem_nonneg; omega.
+  - apply Z.rem_nonneg.
+    omega.
+    pose (Zgt_pos_0 p); omega.
+  - assert (Z.rem (Z.neg p) 100 <= 0) as NONPOS.
+    apply Z.rem_nonpos.
+    omega.
+    pose (Zlt_neg_0 p); omega.
+
+    assert (-100 < Z.rem (Z.neg p) 100).
+    assert (Z.abs (Z.rem (Z.neg p) 100) < Z.abs 100)
+      as BOUND by
+          (apply Z.rem_bound_abs; omega).
+
+    apply Z.abs_lt in BOUND.
+    simpl in BOUND.
+    omega.
+    omega.
+Qed.
+
+Lemma hash_lt_100: forall k, hash k < 100.
+Proof.
+  intro.
+  unfold hash.
+  destruct k;simpl.
+  - apply Z.rem_bound_pos.
+    omega.
+    omega.
+  - apply Z.rem_bound_pos.
+    pose (Zgt_pos_0 p); omega.
+    omega.
+  - assert (100 = 1 + 99) as P0 by omega.
+    rewrite P0 at 2.
+    apply Zplus_lt_compat_r.
+    Check Z.rem_nonpos.
+    SearchAbout Z.rem.
+    Eval compute in (Z.rem (-100) 100).
+    assert (Z.rem (Z.neg p) 100 <= 0) as NONPOS.
+    apply Z.rem_nonpos.
+    omega.
+    pose (Zlt_neg_0 p); omega.
+    omega.
+Qed.    
