coq/verif_assoc.v
@@ -2,40 +2,16 @@ Require Import floyd.proofauto.
 Require Import assoc.
 Require Import assoc_spec.
 Require Import Coq.Logic.FunctionalExtensionality.
+Require Import Psatz.
 
 Local Open Scope logic.
 Local Open Scope Z.
 
+(* Auxillary definitions *)
 Inductive repr : Z -> val -> Prop :=
-| mk_repr : forall z, z >= 0 -> z < Int.modulus -> repr z (Vint (Int.repr z)).
+| mk_repr : forall z, Int.min_signed <= z <= Int.max_signed -> repr z (Vint (Int.repr z)).
 
-Lemma k_in_range: forall k : Z, 0 <= k < 100 -> Int.min_signed <= k <= Int.max_signed.
-Proof.
-  split.
-  unfold Int.min_signed, Int.half_modulus, Int.modulus.
-  unfold Int.wordsize, Wordsize_32.wordsize.
-  unfold two_power_nat.
-  unfold shift_nat.
-  unfold nat_iter.
-  simpl.
-  omega.
-  unfold Int.max_signed, Int.half_modulus, Int.modulus,
-  Int.wordsize, Wordsize_32.wordsize,
-  two_power_nat, shift_nat, nat_iter.
-  simpl; omega.
-Qed.
-
-
-Lemma k_from_val: forall (k:Z) (karg : int), repr k (Vint karg) -> 0 <= k < 100 ->
-                                             Int.signed karg = k.
-Proof.
-intros.
-inversion H.
-apply Int.signed_repr.
-apply k_in_range.
-assumption.
-Qed.
-
+(* Function specifications *)
 Definition get_spec :=
   DECLARE _get
     WITH sh : share, k : Z, arr : ArrayZ, vk : val, varr : val
@@ -66,6 +42,15 @@ Definition set_spec :=
                              (fun x => (Vint (Int.repr (arrGet (arrPut arr k v) x))))
                              0 100 varr).
 
+Definition hash_spec :=
+  DECLARE _hash
+    WITH sh : share, k : Z, vk : val
+    PRE [_key OF tint]
+        PROP ( repr k vk)
+        LOCAL (`(eq vk) (eval_id _key))
+        SEP ()
+    POST [tint] local(`(eq (Vint (Int.repr (hash k)))) retval).
+
 Definition c_get_spec :=
   DECLARE _cGet
     WITH sh : share, k : Z, arr : CircleArrayZ, vk : val, varr : val
@@ -84,8 +69,7 @@ Definition c_set_spec :=
   DECLARE _cSet
      WITH sh : share, k : Z, v : Z, arr : CircleArrayZ, vk : val, vv : val, varr : val
      PRE [_arr OF (tptr tint), _key OF tint, _val OF tint]
-         PROP (writable_share sh; Int.min_signed <= k <= Int.max_signed;
-               repr k vk; Int.min_signed <= v <= Int.max_signed; repr v vv)
+         PROP (writable_share sh; repr k vk; repr v vv)
          LOCAL (`(eq vk) (eval_id _key);
                 `(eq vv) (eval_id _val);
                 `(eq varr) (eval_id _arr);
@@ -98,7 +82,178 @@ Definition c_set_spec :=
                              0 100 varr).
 
 Definition Vprog : varspecs := nil.
-Definition Gprog : funspecs := get_spec :: set_spec :: c_get_spec :: c_set_spec :: nil.
+Definition Gprog : funspecs := get_spec :: set_spec :: hash_spec
+                                        :: c_get_spec :: c_set_spec :: nil.
+
+(* Auxillary lemmas *)
+
+(*
+Lemma k_in_range: forall k : Z, 0 <= k < 100 -> Int.min_signed <= k <= Int.max_signed.
+Proof.
+  split.
+  unfold Int.min_signed, Int.half_modulus, Int.modulus.
+  unfold Int.wordsize, Wordsize_32.wordsize.
+  unfold two_power_nat.
+  unfold shift_nat.
+  unfold nat_iter.
+  simpl.
+  omega.
+  unfold Int.max_signed, Int.half_modulus, Int.modulus,
+  Int.wordsize, Wordsize_32.wordsize,
+  two_power_nat, shift_nat, nat_iter.
+  simpl; omega.
+Qed.
+*)
+
+Lemma k_from_val: forall (k:Z) (karg : int), repr k (Vint karg) -> 0 <= k < 100 ->
+                                             Int.signed karg = k.
+Proof.
+intros.
+inversion H.
+apply Int.signed_repr.
+assumption.
+Qed.
+
+Lemma f_notequal: forall (A B : Type) (f : A -> B) (x y : A), ~ f x = f y -> ~ x = y.
+Proof.
+  pose proof f_equal as FEQ.
+  assert (forall A B:Prop, (A -> B) -> (~B -> ~A)) as CONTRAPOSITION by tauto.
+  intros A B f x y.
+  apply CONTRAPOSITION.
+  apply FEQ.
+Qed.
+
+Lemma neq_100_mone: (Int.eq (Int.repr 100) Int.mone = false).
+Proof.
+  apply Int.eq_false.
+  apply f_notequal with Z Int.intval.
+  simpl.
+  omega.
+Qed.
+
+Lemma neq_100_zero: (Int.eq (Int.repr 100) Int.zero = false).
+Proof.
+  apply Int.eq_false.
+  apply f_notequal with Z Int.intval.
+  simpl.
+  omega.
+Qed.
+
+Lemma hash_bound: forall k, Int.min_signed <= hash k <= Int.max_signed.
+Proof.
+  intro.
+  unfold Int.min_signed, Int.max_signed, Int.half_modulus, Int.modulus, two_power_nat, Int.wordsize, Wordsize_32.wordsize, shift_nat, nat_iter;simpl.
+  split.
+  pose (Zero_le_hash k).
+  omega.
+  pose (hash_lt_100 k).
+  omega.
+Qed.
+
+Lemma Zmod_less: forall a b c, b > 0 -> b <= c -> a mod b < c.
+Proof.
+  intros.
+  assert (forall a b c, a < b -> b <= c -> a < c) as lt_le_trans by (intros; lia).
+  apply lt_le_trans with b.
+  apply Z_mod_lt;auto.
+  assumption.
+Qed.
+
+Lemma body_hash: semax_body Vprog Gprog f_hash hash_spec.
+Proof.
+  start_function.
+  name karg _key.
+  forward_if (PROP (Int.min_signed <= k <= Int.max_signed; repr k vk;
+                    0 <= k)
+                   LOCAL (`(eq vk) (eval_id _key)) SEP()).
+  - forward. rename H into REPRK. rename H0 into KLT0.
+    entailer!.
+    + rewrite neq_100_mone.
+      rewrite andb_false_r.
+      simpl; auto.
+      
+    + unfold force_val, sem_mod, sem_add_default, sem_cast_neutral, sem_binarith.
+      simpl.
+      unfold both_int, sem_cast_neutral.
+      simpl.
+      rewrite neq_100_mone.
+      rewrite andb_false_r.
+      unfold is_int.
+      auto.
+
+    + assert (karg = (Int.repr k)) as KARGEQK by (inv REPRK;tauto).
+      rewrite KARGEQK.
+      unfold force_val, sem_mod, sem_add_default, sem_cast_neutral.
+      unfold sem_binarith, both_int, sem_cast_neutral.
+      simpl.
+      rewrite neq_100_mone.
+      rewrite andb_false_r.
+      simpl.
+      apply f_equal.
+      unfold Int.mods.
+      repeat rewrite Int.signed_repr.
+      rewrite add_repr.
+      apply f_equal.
+      unfold hash.
+      assert (k < 0) as KLESS0.
+      rewrite KARGEQK in KLT0.
+      unfold Int.lt in KLT0.
+      rewrite Int.signed_repr in KLT0.
+      rewrite Int.signed_repr in KLT0.
+      destruct (zlt k 0).
+      assumption.
+      discriminate KLT0.
+      unfold Int.min_signed, Int.max_signed, Int.half_modulus, Int.modulus, two_power_nat, Int.wordsize, Wordsize_32.wordsize, shift_nat, nat_iter.      
+      split;simpl;omega.
+      inv REPRK.
+      assumption.
+      assert ((k <? 0) = true).
+      unfold "<?".
+      unfold "?=".
+      destruct k; [omega|pose (Zgt_pos_0 p);omega|tauto].
+      rewrite H.
+      tauto.
+      unfold Int.min_signed, Int.max_signed, Int.half_modulus, Int.modulus, two_power_nat, Int.wordsize, Wordsize_32.wordsize, shift_nat, nat_iter.
+      split;simpl;omega.
+      inv REPRK;assumption.
+  - forward.
+    entailer. rename H into REPRK.
+    inv REPRK. entailer.
+  - forward.
+    entailer!.
+    + rewrite neq_100_mone.
+      rewrite andb_false_r.
+      simpl.
+      auto.
+    + unfold force_val, sem_mod, sem_add_default, sem_cast_neutral, sem_binarith.
+      simpl.
+      unfold both_int, sem_cast_neutral.
+      simpl.
+      rewrite neq_100_mone.
+      rewrite andb_false_r.
+      unfold is_int.
+      auto.
+    + unfold force_val, sem_mod, sem_add_default, sem_cast_neutral.
+      unfold sem_binarith, both_int, sem_cast_neutral.
+      simpl.
+      rewrite neq_100_mone.
+      rewrite andb_false_r.
+      apply f_equal.
+      unfold Int.mods.
+      repeat rewrite Int.signed_repr.
+      apply f_equal.
+      inv H.
+      rewrite Int.signed_repr.
+      unfold hash.
+      assert ((k <? 0) = false).
+      unfold "<?", "?=".
+      destruct k;[tauto|tauto|pose (Zlt_neg_0 p); omega].
+      rewrite H.
+      tauto.
+      split;assumption.
+      unfold Int.min_signed, Int.max_signed, Int.half_modulus, Int.modulus, two_power_nat, Int.wordsize, Wordsize_32.wordsize, shift_nat, nat_iter.
+      split;simpl;omega.
+Qed.
 
 Lemma body_c_get: semax_body Vprog Gprog f_cGet c_get_spec.
 Proof.
@@ -106,21 +261,35 @@ Proof.
   name karg _key.
   name arrarg _arr.
   name rezloc _rez.
-  forward_call (sh,(Zmod k 100),arr,(Vint (Int.repr (Zmod k 100))), varr).
+  name hloc _h.
+  forward_call (sh,k,vk). (* hash(key) *)
   entailer!.
-  simpl.
+  rewrite <- H1; assumption.
   
-  unfold Int.mone.
-  
-  SearchAbout Int.eq.
-  
-  assert (Int.eq (Int.repr 100) (Int.repr (-1)) = false).
-  apply Int.eq_false.
-  unfold Int.repr.
-  simpl.
-  admit.
 
-  rewrite H2.
+  admit.
+  after_call.
+  forward_call (sh,(hash k),arr,(Vint (Int.repr (hash k))), varr).
+  entailer!. (* get(arr, h) *)
+  - apply Zero_le_hash.
+  - apply hash_lt_100.
+  - apply mk_repr.
+    apply hash_bound.
+  -
+
+  unfold sem_add_default, sem_mod, force_val.
+simpl.  
+  unfold sem_cast_neutral, both_int.
+  rewrite neq_100_mone.
+  rewrite neq_100_zero.
+  simpl.
+  rewrite andb_false_r.
+  unfold denote_tc_nodivover.
+  rewrite neq_100_mone.
+  rewrite andb_false_r.
+  simpl.
+  auto.
+  rewrite neq_100_mone.
   rewrite andb_false_r.
   simpl.
   auto.
@@ -133,18 +302,26 @@ Proof.
   unfold two_power_nat, Int.wordsize.
   unfold Wordsize_32.wordsize, shift_nat.
   unfold nat_iter.
+  apply Zmod_less; omega.
 
-  assert (forall a b c, a < b -> b < c -> a < c) as Lt_Lt_trans by admit.
-  apply Lt_Lt_trans with 100.
-  apply Z_mod_lt; omega.
-  omega.
-  rewrite H1 in H.
-  assert (karg = (Int.repr k)).
-  inv H.
-  tauto.
-  rewrite H2.
+  assert (Vint (Int.repr k) = Vint karg) as kEQkarg by (inv H;assumption).
+  rewrite <- kEQkarg.
   unfold sem_mod.
-  unfold sem_binarith.
+  simpl. 
+  unfold both_int.
+  simpl.
+  rewrite neq_100_mone.
+  rewrite andb_false_r.
+  unfold Int.mods.
+  simpl.
+  rewrite andb_false_r.
+  unfold sem_cast_neutral, force_val.
+  repeat apply f_equal.
+  rewrite add_repr.
+  repeat rewrite Int.signed_repr.
+  apply Zmod_eq_pos_Zrem.
+
+ unfold sem_binarith.
   unfold classify_binarith.
   unfold tint.
   unfold both_int.
@@ -153,24 +330,32 @@ Proof.
   unfold binarith_type.
   unfold sem_cast_neutral.
   simpl.
-  unfold Int.mone.
-  assert (Int.eq (Int.repr 100) (Int.repr (-1)) = false) by admit.
-  rewrite H3.
+  rewrite neq_100_mone.
   rewrite andb_false_r.
   unfold force_val.
-  
   unfold Int.mods.
   rewrite Int.signed_repr.
   rewrite Int.signed_repr.
   repeat apply f_equal.
+
+Eval compute in Z.rem (-5) 100.
+
+  Print Z.modulo.
+  Print Z.pos_div_eucl.
+  Print Z.quotrem.
+
+
   destruct k.
   auto.
   rewrite Zquot.Zrem_Zmod_pos;auto.
-  admit.
+  lia.
   omega.
   unfold Z.rem.
   unfold Z.quotrem.
   unfold Zmod.
+
+Eval compute Z.div_eucl
+
   admit.
   unfold Int.min_signed, Int.max_signed, Int.half_modulus, Int.modulus, two_power_nat, Int.wordsize, Wordsize_32.wordsize, shift_nat, nat_iter.
   simpl.
