coq/intro.v
@@ -1,0 +1,9 @@
+
+Lemma f_inequal: forall (A B : Type) (f : A -> B) (x y : A), ~ f x = f y -> ~ x = y.
+Proof.
+intros A B f x y.
+pose proof f_equal as FEQ.
+assert (forall A B:Prop, (A -> B) -> (~B -> ~A)) by tauto.
+apply H.
+apply FEQ.
+Qed.
